some more progress.

examples/low-level/huffman/huffman.fst
@@ -48,7 +48,7 @@ let rec live_node n sm =
   live_located n sm && liveRef n'.frequency sm && live_node n'.zero_child sm &&
   live_node n'.one_child sm && liveRef n'.code sm
 
-val live_node_after_write: #a:Type -> #b:Type ->  rw:(lref a) -> v:a
+val live_node_after_write: #a:Type ->  rw:(lref a) -> v:a
                            -> n:located node -> m:smem{live_node n m}
                            -> GTot (u:unit{live_node n (writeMemAux rw m v)})
                               (decreases n)
@@ -58,13 +58,30 @@ let rec live_node_after_write rw v n m =
   live_node_after_write rw v n'.zero_child m;
   live_node_after_write rw v n'.one_child m
 
+val live_node_after_salloc: #a:Type -> r:(lref a) -> v:a -> n:located node
+                            -> m:smem{isNonEmpty (st m) /\ not (contains (topstb m) r) /\ live_node n m}
+                            -> GTot (u:unit{live_node n (allocateInTopR r v m)})
+                               (decreases n)
+let rec live_node_after_salloc r v n m =
+  greveal_precedence_axiom n;
+  let n' = greveal n in
+  live_node_after_salloc r v n'.zero_child m;
+  live_node_after_salloc r v n'.one_child m
+
 (* TODO: FIXME: Can't write ghost code in lemmas *)
-val live_node_after_write_lemma: #a:Type -> #b:Type ->  rw:(lref a) -> v:a
+val live_node_after_write_lemma: #a:Type -> rw:(lref a) -> v:a
                                  -> n:located node -> m:smem{live_node n m}
                                  -> Lemma (requires (True))
                                           (ensures (live_node n (writeMemAux rw m v)))
-                                    [SMTPat (writeMemAux rw m v)]
+                                    [SMTPat (writeMemAux rw m v); SMTPat (live_node n m)]
 let live_node_after_write_lemma rw v n m = admit ()
+
+val live_node_after_salloc_lemma: #a:Type -> r:(lref a) -> v:a -> n:located node
+                            -> m:smem{isNonEmpty (st m) /\ not (contains (topstb m) r) /\ live_node n m}
+                            -> Lemma (requires (True))
+                                     (ensures (live_node n (allocateInTopR r v m)))
+                               [SMTPat (allocateInTopR r v m); SMTPat (live_node n m)]
+let live_node_after_salloc_lemma r v n m = admit ()
 
 (* projectors *)
 assume val read_frequency: n:located node -> PureMem (lref int)
@@ -119,14 +136,23 @@ let rec live_list l sm = match l with
   | []     -> true
   | hd::tl -> live_node hd sm && live_list tl sm
 
-val live_list_after_write_lemma: #a:Type -> #b:Type ->  rw:(lref a) -> v:a
+val live_list_after_write_lemma: #a:Type -> rw:(lref a) -> v:a
                                  -> l:list (located node) -> m:smem{live_list l m}
                                  -> Lemma (requires (True))
                                           (ensures (live_list l (writeMemAux rw m v)))
-                                    [SMTPat (writeMemAux rw m v)]
+                                    [SMTPat (writeMemAux rw m v); SMTPat (live_list l m)]
 let rec live_list_after_write_lemma rw v l m = match l with
   | []     -> ()
   | hd::tl -> live_list_after_write_lemma rw v tl m
+
+val live_list_after_salloc_lemma: #a:Type -> r:(lref a) -> v:a -> l:list (located node)
+                            -> m:smem{isNonEmpty (st m) /\ not (contains (topstb m) r) /\ live_list l m}
+                            -> Lemma (requires (True))
+                                     (ensures (live_list l (allocateInTopR r v m)))
+                               [SMTPat (allocateInTopR r v m); SMTPat (live_list l m)]
+let rec live_list_after_salloc_lemma r v l m = match l with
+  | []     -> ()
+  | hd::tl -> live_list_after_salloc_lemma r v tl m
 
 val live_node_list: l:node_list -> sm:smem -> GTot bool
 let live_node_list l sm = liveRef l sm && live_list (loopkupRef l sm) sm
@@ -200,6 +226,109 @@ val insert_in_ordered_node_list:
 let insert_in_ordered_node_list n l =
   let r = insert_in_ordered_list n (memread l) in
   memwrite l r
+
+(**********)
+
+type data = sstarray symbol_t
+
+type histogram = sstarray (located node)
+
+val live_histogram_arr: h:sstarray (located node) -> sm:smem{liveArr sm h}
+                        -> i:nat{i <= glength h sm}
+                        -> GTot (r:bool{r ==> (forall (j:nat). (j >= i /\ j < glength h sm) ==> live_node (gindex h sm j) sm)})
+                           (decreases (glength h sm - i))
+let rec live_histogram_arr h sm i =
+  if i = glength h sm then true
+  else
+    live_node (gindex h sm i) sm && live_histogram_arr h sm (i + 1)
+
+val live_hist_arr_after_write: #a:Type -> rw:(lref a) -> v:a
+                           -> h:histogram{reveal (asRef h) =!= rw} -> i:nat
+                           -> m:smem{liveArr m h /\ i <= glength h m /\ live_histogram_arr h m i}
+                           -> m':smem{m' = writeMemAux rw m v}
+                           -> GTot (u:unit{liveArr m' h /\ i <= glength h m' /\ live_histogram_arr h m' i})
+                              (decreases (glength h m - i))
+let rec live_hist_arr_after_write rw v h i m m' =
+  if i = glength h m then ()
+  else live_hist_arr_after_write rw v h (i + 1) m m'
+
+val live_hist_arr_after_salloc: #a:Type -> r:(lref a) -> v:a -> h:histogram{reveal (asRef h) =!= r} -> i:nat
+                            -> m:smem{isNonEmpty (st m) /\ not (contains (topstb m) r) /\
+                                      liveArr m h /\ i <= glength h m /\ live_histogram_arr h m i}
+                            -> m':smem{m' = allocateInTopR r v m}
+                            -> GTot (u:unit{liveArr m' h /\ i <= glength h m' /\ live_histogram_arr h m' i})
+                               (decreases (glength h m - i))
+let rec live_hist_arr_after_salloc r v h i m m' =
+  if i = glength h m then ()
+  else live_hist_arr_after_salloc r v h (i + 1) m m'
+
+val live_hist_arr_after_write_lemma: #a:Type -> rw:(lref a) -> v:a
+                           -> h:histogram{reveal (asRef h) =!= rw} -> i:nat
+                           -> m:smem{liveArr m h /\ i <= glength h m /\ live_histogram_arr h m i}
+                           -> m':smem{m' = writeMemAux rw m v}
+                           -> Lemma (requires (True))
+                              (ensures (liveArr m' h /\ i <= glength h m' /\ live_histogram_arr h m' i))
+                              [SMTPat (live_histogram_arr h m i); SMTPat (live_histogram_arr h m' i); SMTPat (writeMemAux rw m v)]
+let live_hist_arr_after_write_lemma rw v h i m m' = admit ()
+
+val live_hist_arr_after_salloc_lemma: #a:Type -> r:(lref a) -> v:a -> h:histogram{reveal (asRef h) =!= r} -> i:nat
+                            -> m:smem{isNonEmpty (st m) /\ not (contains (topstb m) r) /\
+                                      liveArr m h /\ i <= glength h m /\ live_histogram_arr h m i}
+                            -> m':smem{m' = allocateInTopR r v m}
+                            -> Lemma (requires (True))
+                               (ensures (liveArr m' h /\ i <= glength h m' /\ live_histogram_arr h m' i))
+                               [SMTPat (live_histogram_arr h m i); SMTPat (live_histogram_arr h m' i); SMTPat (allocateInTopR r v m)]
+let live_hist_arr_after_salloc_lemma r v h i m m' = admit ()
+
+val live_histogram: h:histogram -> sm:smem -> GTot (r:bool{r ==> (liveArr sm h /\
+                                                                  (forall i. (i >= 0 /\ i < glength h sm) ==>
+                                                                              live_node (gindex h sm i) sm))})
+let live_histogram h sm = liveArr sm h && live_histogram_arr h sm 0
+
+val live_hist_after_write_lemma: #a:Type -> rw:(lref a) -> v:a
+                           -> h:histogram{reveal (asRef h) =!= rw}
+                           -> m:smem{live_histogram h m}
+                           -> m':smem{m' = writeMemAux rw m v}
+                           -> Lemma (requires (True))
+                              (ensures (live_histogram h m'))
+                              [SMTPat (live_histogram h m); SMTPat (live_histogram h m'); SMTPat (writeMemAux rw m v)]                              
+let live_hist_after_write_lemma rw v h m m' = ()
+
+val live_hist_after_salloc_lemma: #a:Type -> r:(lref a) -> v:a -> h:histogram{reveal (asRef h) =!= r}
+                            -> m:smem{isNonEmpty (st m) /\ not (contains (topstb m) r) /\
+                                      live_histogram h m}
+                            -> m':smem{m' = allocateInTopR r v m}
+                            -> Lemma (requires (True))
+                               (ensures (live_histogram h m'))
+                               [SMTPat (live_histogram h m); SMTPat (live_histogram h m'); SMTPat (allocateInTopR r v m)]
+let live_hist_after_salloc_lemma r v h m m' = ()
+
+val compute_histogram: d:data -> h:histogram -> i:nat
+                       -> SST unit
+                          (fun m0 -> isNonEmpty (st m0)                        /\
+                                     liveArr m0 d /\ live_histogram h m0       /\
+                                     glength h m0 = symbol_value_bound /\
+                                     i <= glength d m0)
+                          (fun m0 r m1 -> isNonEmpty (st m0)                        /\
+                                          liveArr m0 d /\ live_histogram h m0       /\
+                                          glength h m0 = symbol_value_bound /\
+                                          i <= glength d m0 /\ isNonEmpty (st m1))
+                                                                   (*/\
+                                          isNonEmpty (st m1))*)
+                                                                 (*/\
+                                          liveArr m1 d ) /\ live_histogram h m1)*)
+let compute_histogram d h i =
+  if i = SSTArray.length d then ()
+  else
+    let sym = SSTArray.readIndex d i in    
+    let the_leaf = SSTArray.readIndex h sym in
+    if is_null the_leaf then
+      let the_leaf' = mk_node (salloc 1) (mk_null_node ()) (mk_null_node ()) sym (salloc "") in
+      SSTArray.writeIndex h sym the_leaf'
+    else admit ()
+      //memwrite (the_leaf.frequency) ((memread the_leaf.frequency) + 1)
+
+
 
 (*val insert_in_ordered_list: n:located node -> l:node_list
                             -> SST unit
